Incremental/FreeTheorem.lean
@@ -10,37 +10,6 @@ variable {ℭ : BuildConfig} {q₀ α}
 
 namespace Task
 
-namespace Monad
-
-structure Action (κ₁ κ₂ : Type → Type) [Monad κ₁] [Monad κ₂] where
-  rel {α β : Type} :
-    (α → β → Prop) →
-    (κ₁ α → κ₂ β → Prop)
-  rel_pure {α β : Type} {R : α → β → Prop} {a : α} {b : β} :
-    R a b → rel R (pure a) (pure b)
-  rel_bind
-    {α₁ α₂ β₁ β₂ : Type}
-    {R : α₁ → α₂ → Prop} {S : β₁ → β₂ → Prop}
-    {ma : κ₁ α₁} {mb : κ₂ α₂}
-    {ka : α₁ → κ₁ β₁} {kb : α₂ → κ₂ β₂} :
-    rel R ma mb →
-    (∀ a b, R a b → rel S (ka a) (kb b)) →
-    rel S (ma >>= ka) (mb >>= kb)
-
-axiom freeTheorem
-    {κ₁ κ₂ : Type → Type} [Monad κ₁] [Monad κ₂]
-    (t : Task Monad ℭ q₀ α)
-    (F : Action κ₁ κ₂)
-    (ι₁ : ∀ i, κ₁ (ℭ.V i))
-    (ι₂ : ∀ i, κ₂ (ℭ.V i))
-    (fetch₁ : ∀ q, ℭ.rel q q₀ → κ₁ (ℭ.R q))
-    (fetch₂ : ∀ q, ℭ.rel q q₀ → κ₂ (ℭ.R q))
-    (hι : ∀ i, F.rel Eq (ι₁ i) (ι₂ i))
-    (hfetch : ∀ q hq, F.rel Eq (fetch₁ q hq) (fetch₂ q hq)) :
-    F.rel Eq (t κ₁ ι₁ fetch₁) (t κ₂ ι₂ fetch₂)
-
-end Monad
-
 namespace Applicative
 
 structure Action (κ₁ κ₂ : Type → Type) [Applicative κ₁] [Applicative κ₂] where
@@ -88,23 +57,6 @@ theorem Tasks.Applicative.freeTheorem
     (fun q _ => compute (inferInstance : Applicative Id) tasks ι₀ q) hι hfetch
   have heval : tasks q₀ Id ι₀ (fun q _ => compute (inferInstance : Applicative Id) tasks ι₀ q) =
       compute (inferInstance : Applicative Id) tasks ι₀ q₀ := by
-    conv => rhs; unfold compute
-  simpa only [heval] using h
-
-theorem Tasks.Monad.freeTheorem
-    {κ : Type → Type} [Monad κ]
-    (tasks : Tasks Monad ℭ) (q₀ : ℭ.Q)
-    (F : Task.Monad.Action κ Id)
-    (ι₀ : ∀ i, ℭ.V i)
-    (ι₁ : ∀ i, κ (ℭ.V i))
-    (fetch₁ : ∀ q, ℭ.rel q q₀ → κ (ℭ.R q))
-    (hι : ∀ i, F.rel Eq (ι₁ i) (ι₀ i))
-    (hfetch : ∀ q hq, F.rel Eq (fetch₁ q hq) (computeM tasks ι₀ q)) :
-    F.rel Eq (tasks q₀ κ ι₁ fetch₁) (computeM tasks ι₀ q₀) := by
-  have h := Task.Monad.freeTheorem (tasks q₀) F ι₁ ι₀ fetch₁
-    (fun q _ => computeM tasks ι₀ q) hι hfetch
-  have heval : tasks q₀ Id ι₀ (fun q _ => computeM tasks ι₀ q) =
-      computeM tasks ι₀ q₀ := by
     conv => rhs; unfold compute
   simpa only [heval] using h
 
